added fupdate_NORMALISE_CONV
fupdate_NORMALISE_CONV simplifies fupdate - sequences by removing the ones that are masked by
later appearances. 

``f |+ (x1, y1) |+ (x2, y2) |+ (x1, y3) |+ (x4, y4)``
gets for example simplied to to

   |- (f |+ (x1, y1) |+ (x2, y2) |+ (x1, y3) |+ (x4, y4)) =
      (f |+             (x2, y2) |+ (x1, y3) |+ (x4, y4))

The slightly tricky part in writing this conversion was to avoid checking, whether two keys are equal. 
They are treaded as equal by this conversion, iff they are alpha-equivalent. Otherwise, it is not 
somehow cleverly checked, whether they are equal. 

For implementing this conversion the concept of two finite maps beeing equal upto a given
set of keys (fmap_EQ_UPTO) was introduced in finite_mapTheory.

src/finite_map/finite_mapLib.sig
@@ -20,4 +20,17 @@ sig
   val fevery_EXPAND_CONV : Abbrev.conv
 
 
+  (*Simplies fupdate - sequences by removing the ones that are masked by
+    later appearances.
+
+  ``f |+ (x1, y1) |+ (x2, y2) |+ (x1, y3) |+ (x4, y4)``
+
+  gets for example simplied to to
+
+   |- (f |+ (x1, y1) |+ (x2, y2) |+ (x1, y3) |+ (x4, y4)) =
+      (f |+             (x2, y2) |+ (x1, y3) |+ (x4, y4))
+
+  *)
+  val fupdate_NORMALISE_CONV : Abbrev.conv
+
 end
