src/finite_map/finite_mapLib.sml
@@ -5,7 +5,7 @@ struct
 
   val ERR = mk_HOL_ERR "finite_mapLib"
 
-  local open finite_mapTheory finite_mapSyntax pred_setTheory in
+  local open finite_mapTheory finite_mapSyntax pred_setTheory simpLib in
 
 
 val FEVERY_cs = computeLib.bool_compset ()
@@ -26,8 +26,61 @@ end;
 
 
 
+
+local
+   fun add_fup ([], []) kL2 thm = thm
+     | add_fup (k::kL, v::vL) kL2 thm =
+       let
+          val c = concl thm
+          val ks = rand c
+          val f2 = (rand o rator) c
+          val f1 = (rand o rator o rator) c
+
+          val (kL2, inkL2) = (snd (Lib.pluck (fn x => x = k) kL2), true) handle HOL_ERR _ =>
+                             (kL2, false)
+          val inkL = mem k kL
+          val kL2 = if inkL then k::kL2 else kL2;
+          val imp_thm = if inkL then fmap_EQ_UPTO___FUPDATE_SING else
+               if inkL2 then
+                  fmap_EQ_UPTO___FUPDATE_BOTH
+               else
+                  fmap_EQ_UPTO___FUPDATE_BOTH___NO_DELETE
+
+          val imp_thm_inst = ISPECL [f1,f2, ks, k, v] imp_thm
+          val thm1 = MP imp_thm_inst thm
+
+       in
+          add_fup (kL, vL) kL2 thm1
+       end
+     | add_fup _ kL2 thm = Feedback.fail ();
+
+   val emp_conv =
+        simpLib.SIMP_CONV (boolSimps.bool_ss++boolSimps.CONJ_ss) [EXTENSION, NOT_IN_EMPTY, IN_DELETE, IN_INSERT]
+in
+
+
+fun fupdate_NORMALISE_CONV t = 
+let
+   val (base, kvL) = strip_fupdate t
+   val (kL,vL) = unzip (map pairSyntax.dest_pair kvL)
+
+
+   val typed_empty_tm = 
+        Term.inst [alpha |-> fst (finite_mapSyntax.dest_fmap_ty (type_of base))] pred_setSyntax.empty_tm
+
+
+   val thm0 = ISPECL [typed_empty_tm, base] fmap_EQ_UPTO___EQ
+   val thm1 = add_fup (kL, vL) [] thm0
+   val emp_thm = EQT_ELIM (emp_conv (mk_eq ((rand o concl) thm1, typed_empty_tm)));
+
+   val thm2 = CONV_RULE (RAND_CONV (K emp_thm) THENC
+                         REWR_CONV fmap_EQ_UPTO___EMPTY) thm1
+in
+   thm2
 end;
+
 end;
 
+end;
 
-
+end;
